Uncheat pure_to_thunkProof

compiler/backend/proofs/pure_to_thunkProofScript.sml
@@ -5,7 +5,7 @@
 open HolKernel Parse boolLib bossLib term_tactic monadsyntax;
 open stringTheory optionTheory sumTheory pairTheory listTheory alistTheory
      finite_mapTheory pred_setTheory rich_listTheory thunkLang_substTheory
-     pure_evalTheory thunkLang_primitivesTheory
+     pure_evalTheory thunkLang_primitivesTheory dep_rewrite;
 open pure_exp_lemmasTheory pure_miscTheory;
 
 val _ = new_theory "pure_to_thunkProof";
@@ -46,6 +46,7 @@ val _ = numLib.prefer_num ();
       semantics).
     - The remainder of the operations already produce results in weak head
       normal form, so we don't do anything special to them.
+    - The first argument to ‘Seq’ is forced.
   * [Letrec]
     - We expect all expressions in the list of bindings to be suspended by
       something (either Lam or Delay or Box), so we insert Delay everywhere.
@@ -106,9 +107,16 @@ Inductive exp_rel:
   (∀s i xs ys.
      LIST_REL exp_rel xs ys ⇒
        exp_rel (Prim (Proj s i) xs) (Force (Prim (Proj s i) ys))) ∧
+[exp_rel_Seq:]
+  (∀x1 x2 y1 y2.
+     LIST_REL exp_rel [x1; y1] [x2; y2] ∧
+     closed x1 ∧
+     s ∉ freevars y1 ⇒
+       exp_rel (Seq x1 y1) (Let s x2 y2)) ∧
 [exp_rel_Prim:]
   (∀op xs ys.
      op ≠ If ∧
+     op ≠ Seq ∧
      (∀n. op ≠ Cons n) ∧
      (∀s i. op ≠ Proj s i) ∧
      LIST_REL exp_rel xs ys ⇒
@@ -193,6 +201,80 @@ Proof
   \\ imp_res_tac pure_expTheory.exp_size_lemma \\ fs []
 QED
 
+Theorem exp_rel_freevars:
+  ∀x y. exp_rel x y ⇒ freevars x = freevars y
+Proof
+  ho_match_mp_tac exp_rel_ind \\ rw []
+  \\ fs [freevars_def, pure_expTheory.closed_def, DELETE_DEF,
+         AC UNION_COMM UNION_ASSOC, MAP_MAP_o, combinTheory.o_DEF]
+  >- (
+    ‘freevars x = EMPTY’
+      by (drule_then (qspec_then ‘REVERSE f’ mp_tac) ALOOKUP_SOME_EL_2
+          \\ impl_tac
+          >- (
+            last_x_assum mp_tac
+            \\ rpt (pop_assum kall_tac)
+            \\ qid_spec_tac ‘g’
+            \\ Induct_on ‘f’ \\ Cases_on ‘g’ \\ simp [ELIM_UNCURRY])
+          \\ rw [] \\ gvs [EL_REVERSE, LIST_REL_EL_EQN]
+          \\ qmatch_asmsub_abbrev_tac ‘EL m f’
+          \\ ‘m < LENGTH g’ by fs [Abbr ‘m’]
+          \\ first_x_assum (drule_then assume_tac) \\ gs [])
+    \\ fs []
+    \\ qsuff_tac ‘∀x. x ∈ set (MAP (λ(fn,e). freevars e) f) ⇒ x = EMPTY’
+    >- (
+      rw [EXTENSION]
+      \\ fs [MEM_MAP, PULL_EXISTS]
+      \\ rw [DISJ_EQ_IMP]
+      \\ pairarg_tac \\ gvs [])
+    \\ simp [MEM_MAP, MEM_EL]
+    \\ once_rewrite_tac [EQ_SYM_EQ]
+    \\ rw [] \\ pairarg_tac \\ gvs []
+    \\ gvs [LIST_REL_EL_EQN]
+    \\ first_x_assum (drule_then assume_tac)
+    \\ pairarg_tac \\ gvs []
+    \\ pairarg_tac \\ gvs [])
+  >- (
+    pop_assum mp_tac
+    \\ qid_spec_tac ‘ys’
+    \\ Induct_on ‘xs’ \\ Cases_on ‘ys’ \\ simp [] \\ rw []
+    \\ res_tac \\ fs [])
+  >- (
+    pop_assum mp_tac
+    \\ qid_spec_tac ‘ys’
+    \\ Induct_on ‘xs’ \\ Cases_on ‘ys’ \\ simp [] \\ rw []
+    \\ res_tac \\ fs [])
+  >- (
+    rw [EXTENSION, EQ_IMP_THM]
+    \\ strip_tac \\ gs [])
+  >- (
+    pop_assum mp_tac
+    \\ qid_spec_tac ‘ys’
+    \\ Induct_on ‘xs’ \\ Cases_on ‘ys’ \\ simp [] \\ rw []
+    \\ res_tac \\ fs [])
+  >- (
+    ‘MAP FST f = MAP FST g’
+      by (qpat_x_assum ‘LIST_REL _ _ _’ mp_tac
+          \\ rpt (pop_assum kall_tac)
+          \\ qid_spec_tac ‘g’
+          \\ Induct_on ‘f’ \\ Cases_on ‘g’ \\ simp [ELIM_UNCURRY])
+    \\ fs []
+    \\ simp [MAP_MAP_o, combinTheory.o_DEF, LAMBDA_PROD, freevars_def,
+             GSYM pure_miscTheory.FST_THM]
+    \\ rpt (AP_THM_TAC ORELSE AP_TERM_TAC)
+    \\ last_x_assum mp_tac
+    \\ rpt (pop_assum kall_tac)
+    \\ qid_spec_tac ‘g’
+    \\ Induct_on ‘f’ \\ Cases_on ‘g’ \\ fs [ELIM_UNCURRY])
+QED
+
+Theorem exp_rel_closed:
+  exp_rel x y ⇒ closed x = closed y
+Proof
+  metis_tac [closed_def, pure_expTheory.closed_def, exp_rel_freevars,
+             pure_miscTheory.NIL_iff_NOT_MEM]
+QED
+
 Theorem exp_rel_subst:
   ∀x y a b n s.
     exp_rel x y ∧
@@ -229,6 +311,14 @@ Proof
       \\ gvs [LIST_REL_EL_EQN] \\ rw []
       \\ first_x_assum irule \\ fs [MEM_EL]
       \\ irule_at Any EQ_REFL \\ fs [])
+    >- ((* Seq *)
+      simp [subst_single_def, subst1_def]
+      \\ IF_CASES_TAC \\ gvs [subst_ignore_single]
+      \\ irule exp_rel_Seq \\ fs []
+      \\ ‘closed (Tick a)’ by fs [pure_expTheory.closed_def]
+      \\ fs [freevars_subst_single, SF DNF_ss]
+      \\ last_x_assum (irule_at Any) \\ fs []
+      \\ last_assum (irule_at Any) \\ fs [])
     >- ((* Others *)
       simp [subst_single_def, subst1_def]
       \\ rw [Once exp_rel_cases, EVERY2_MAP]
@@ -285,77 +375,6 @@ Proof
     \\ first_assum (irule_at Any) \\ fs []
     \\ first_x_assum (drule_all_then assume_tac)
     \\ pairarg_tac \\ gvs [])
-QED
-
-Theorem exp_rel_freevars:
-  ∀x y. exp_rel x y ⇒ freevars x = freevars y
-Proof
-  ho_match_mp_tac exp_rel_ind \\ rw []
-  \\ fs [freevars_def, pure_expTheory.closed_def, DELETE_DEF,
-         AC UNION_COMM UNION_ASSOC, MAP_MAP_o, combinTheory.o_DEF]
-  >- (
-    ‘freevars x = EMPTY’
-      by (drule_then (qspec_then ‘REVERSE f’ mp_tac) ALOOKUP_SOME_EL_2
-          \\ impl_tac
-          >- (
-            last_x_assum mp_tac
-            \\ rpt (pop_assum kall_tac)
-            \\ qid_spec_tac ‘g’
-            \\ Induct_on ‘f’ \\ Cases_on ‘g’ \\ simp [ELIM_UNCURRY])
-          \\ rw [] \\ gvs [EL_REVERSE, LIST_REL_EL_EQN]
-          \\ qmatch_asmsub_abbrev_tac ‘EL m f’
-          \\ ‘m < LENGTH g’ by fs [Abbr ‘m’]
-          \\ first_x_assum (drule_then assume_tac) \\ gs [])
-    \\ fs []
-    \\ qsuff_tac ‘∀x. x ∈ set (MAP (λ(fn,e). freevars e) f) ⇒ x = EMPTY’
-    >- (
-      rw [EXTENSION]
-      \\ fs [MEM_MAP, PULL_EXISTS]
-      \\ rw [DISJ_EQ_IMP]
-      \\ pairarg_tac \\ gvs [])
-    \\ simp [MEM_MAP, MEM_EL]
-    \\ once_rewrite_tac [EQ_SYM_EQ]
-    \\ rw [] \\ pairarg_tac \\ gvs []
-    \\ gvs [LIST_REL_EL_EQN]
-    \\ first_x_assum (drule_then assume_tac)
-    \\ pairarg_tac \\ gvs []
-    \\ pairarg_tac \\ gvs [])
-  >- (
-    pop_assum mp_tac
-    \\ qid_spec_tac ‘ys’
-    \\ Induct_on ‘xs’ \\ Cases_on ‘ys’ \\ simp [] \\ rw []
-    \\ res_tac \\ fs [])
-  >- (
-    pop_assum mp_tac
-    \\ qid_spec_tac ‘ys’
-    \\ Induct_on ‘xs’ \\ Cases_on ‘ys’ \\ simp [] \\ rw []
-    \\ res_tac \\ fs [])
-  >- (
-    pop_assum mp_tac
-    \\ qid_spec_tac ‘ys’
-    \\ Induct_on ‘xs’ \\ Cases_on ‘ys’ \\ simp [] \\ rw []
-    \\ res_tac \\ fs [])
-  >- (
-    ‘MAP FST f = MAP FST g’
-      by (qpat_x_assum ‘LIST_REL _ _ _’ mp_tac
-          \\ rpt (pop_assum kall_tac)
-          \\ qid_spec_tac ‘g’
-          \\ Induct_on ‘f’ \\ Cases_on ‘g’ \\ simp [ELIM_UNCURRY])
-    \\ fs []
-    \\ simp [MAP_MAP_o, combinTheory.o_DEF, LAMBDA_PROD, freevars_def,
-             GSYM pure_miscTheory.FST_THM]
-    \\ rpt (AP_THM_TAC ORELSE AP_TERM_TAC)
-    \\ last_x_assum mp_tac
-    \\ rpt (pop_assum kall_tac)
-    \\ qid_spec_tac ‘g’
-    \\ Induct_on ‘f’ \\ Cases_on ‘g’ \\ fs [ELIM_UNCURRY])
-QED
-
-Theorem exp_rel_closed:
-  exp_rel x y ⇒ closed x = closed y
-Proof
-  metis_tac [closed_def, pure_expTheory.closed_def, exp_rel_freevars,
-             pure_miscTheory.NIL_iff_NOT_MEM]
 QED
 
 Theorem closed_Delay[local,simp]:
@@ -420,6 +439,56 @@ Proof
       irule exp_rel_Proj
       \\ fs [EVERY2_MAP, LIST_REL_EL_EQN]
       \\ rw [] \\ gvs [EL_MEM])
+    >- ((* Seq *)
+      irule exp_rel_Seq \\ fs []
+      \\ conj_tac
+      >- (
+        DEP_REWRITE_TAC [freevars_subst] \\ fs []
+        \\ simp [FRANGE_FLOOKUP, flookup_fupdate_list, GSYM MAP_REVERSE,
+                 GSYM FILTER_REVERSE, ALOOKUP_MAP, ALOOKUP_FILTER]
+        \\ rw []
+        \\ gvs [CaseEq "option"]
+        \\ imp_res_tac ALOOKUP_SOME_EL
+        \\ gvs [EL_REVERSE, LIST_REL_EL_EQN]
+        \\ qmatch_asmsub_abbrev_tac ‘EL m f’
+        \\ ‘m < LENGTH g’ by fs [Abbr ‘m’]
+        \\ first_assum (drule_then assume_tac)
+        \\ rpt (pairarg_tac \\ fs [])
+        \\ gvs [pure_expTheory.closed_def]
+        \\ rw [EVERY_MAP, EVERY_EL]
+        \\ first_x_assum (drule_then assume_tac)
+        \\ rpt (pairarg_tac \\ fs []))
+      \\ fs [SF DNF_ss]
+      \\ qmatch_goalsub_abbrev_tac ‘MAP f1 (FILTER _ gg)’
+      \\ ‘FILTER (λ(n,v). n ≠ s) (MAP f1 (FILTER (λ(n,x). n ∉ ks) gg)) =
+          MAP f1 (FILTER (λ(m,x). m ∉ ks ∪ {s}) gg)’
+        by (simp [FILTER_MAP, combinTheory.o_DEF, FILTER_FILTER, LAMBDA_PROD,
+                  Abbr ‘f1’]
+            \\ rpt (AP_TERM_TAC ORELSE AP_THM_TAC)
+            \\ rw [FUN_EQ_THM, EQ_IMP_THM])
+      \\ pop_assum SUBST_ALL_TAC
+      \\ unabbrev_all_tac
+      \\ first_x_assum (irule_at Any) \\ fs []
+      \\ first_assum (irule_at Any) \\ fs []
+      \\ qmatch_goalsub_abbrev_tac ‘MAP f1 (FILTER _ gg)’
+      \\ ‘subst (FEMPTY |++ MAP f1 (FILTER (λ(m,x). m ∉ ks) gg)) y1 =
+          subst (FEMPTY |++ MAP f1 (FILTER (λ(m,x). m ∉ ks ∪ {s}) gg)) y1’
+        by (qmatch_goalsub_abbrev_tac ‘subst m2 _ = _’
+            \\ drule_then (qspec_then ‘m2’ mp_tac) subst_fdomsub
+            \\ strip_tac \\ unabbrev_all_tac
+            \\ pop_assum SUBST1_TAC
+            \\ rpt (AP_TERM_TAC ORELSE AP_THM_TAC)
+            \\ simp [DOMSUB_FUPDATE_LIST, combinTheory.o_DEF, FILTER_MAP,
+                     LAMBDA_PROD, FILTER_FILTER]
+            \\ rpt (AP_TERM_TAC ORELSE AP_THM_TAC)
+            \\ rw [FUN_EQ_THM, EQ_IMP_THM])
+      \\ pop_assum SUBST_ALL_TAC
+      \\ qmatch_goalsub_abbrev_tac ‘FILTER f2 (MAP _ _)’
+      \\ ‘f2 = λ(m,x). m ∉ ks ∪ {s}’ by fs []
+      \\ pop_assum SUBST_ALL_TAC
+      \\ pop_assum kall_tac
+      \\ unabbrev_all_tac
+      \\ first_assum (irule_at Any) \\ fs [])
     \\ irule exp_rel_Prim
     \\ fs [EVERY2_MAP, LIST_REL_EL_EQN]
     \\ rw [] \\ gvs [EL_MEM])
@@ -589,6 +658,27 @@ Proof
   \\ simp [FILTER_T, GSYM LAMBDA_PROD]
 QED
 
+Theorem subst1_fresh:
+  ∀x s v.
+    s ∉ freevars x ⇒ subst1 s v x = x
+Proof
+  ho_match_mp_tac freevars_ind \\ rw []
+  \\ fs [freevars_def, subst1_def]
+  >- (
+    irule MAP_ID_ON \\ rw []
+    \\ first_x_assum irule
+    \\ gs [MEM_MAP, Once DISJ_COMM, DISJ_EQ_IMP, PULL_EXISTS])
+  \\ IF_CASES_TAC \\ fs []
+  \\ irule MAP_ID_ON \\ simp [FORALL_PROD]
+  \\ qx_genl_tac [‘k’, ‘y’] \\ strip_tac
+  \\ fs [MEM_MAP, FORALL_PROD, Once DISJ_COMM, DISJ_EQ_IMP, EXISTS_PROD,
+         PULL_EXISTS]
+  \\ first_x_assum irule
+  \\ first_assum (irule_at Any)
+  \\ first_assum (irule_at Any)
+  \\ first_assum (irule_at Any)
+QED
+
 Theorem exp_rel_eval_to:
   ∀k x res y.
     eval_wh_to k x = res ∧
@@ -692,19 +782,16 @@ Proof
       \\ Cases_on ‘op’ \\ fs [LIST_REL_EL_EQN]
       >- (
         IF_CASES_TAC \\ gvs [LENGTH_EQ_NUM_compute])
+      \\ Cases_on ‘xs = []’ \\ fs [get_atoms_def, LIST_REL_EL_EQN, map_def]
       >- (
-        Cases_on ‘xs = []’ \\ fs [get_atoms_def, LIST_REL_EL_EQN, map_def]
-        >- (
-          CASE_TAC \\ fs []
-          \\ CASE_TAC \\ fs []
-          \\ IF_CASES_TAC \\ fs [])
-        \\ ‘ys ≠ []’ by (strip_tac \\ fs [])
-        \\ qmatch_goalsub_abbrev_tac ‘map f ys’
-        \\ ‘f = K (INL Diverge)’ by rw [combinTheory.K_DEF]
-        \\ pop_assum SUBST_ALL_TAC
-        \\ simp [map_K_INL, get_atoms_MAP_Diverge])
-      \\ simp [MEM_MAP]
-      \\ cheat (* TODO No Seq *))
+        CASE_TAC \\ fs []
+        \\ CASE_TAC \\ fs []
+        \\ IF_CASES_TAC \\ fs [])
+      \\ ‘ys ≠ []’ by (strip_tac \\ fs [])
+      \\ qmatch_goalsub_abbrev_tac ‘map f ys’
+      \\ ‘f = K (INL Diverge)’ by rw [combinTheory.K_DEF]
+      \\ pop_assum SUBST_ALL_TAC
+      \\ simp [map_K_INL, get_atoms_MAP_Diverge])
     \\ rw [Once exp_rel_cases]
     >- ((* If *)
       simp [eval_to_def, eval_wh_to_def]
@@ -748,6 +835,17 @@ Proof
       \\ IF_CASES_TAC \\ gvs []
       \\ first_x_assum (drule_then assume_tac)
       \\ fs [thunk_rel_def, dest_anyThunk_def, subst_funs_def, bind_def])
+    >- ((* Seq *)
+      drule_then assume_tac exp_rel_freevars \\ fs []
+      \\ simp [eval_wh_to_def, eval_to_def]
+      \\ simp [subst_funs_def, bind_def]
+      \\ fs [SF DNF_ss]
+      \\ first_assum (drule_then assume_tac) \\ fs []
+      \\ qpat_x_assum ‘exp_rel x1 _’ assume_tac
+      \\ first_x_assum (drule_then assume_tac) \\ fs []
+      \\ simp [subst1_fresh]
+      \\ IF_CASES_TAC \\ gvs []
+      \\ Cases_on ‘eval_to (k - 1) x2’ \\ fs [])
     >- ((* {IsEq, AtomOp, Lit} *)
       simp [eval_wh_to_def, eval_to_def]
       \\ gvs [LIST_REL_EL_EQN, eval_to_def]
@@ -860,11 +958,7 @@ Proof
         \\ ‘exp_rel (EL x xs) (EL x ys) ∧ MEM (EL x xs) xs’
           by fs [EL_MEM]
         \\ last_x_assum (drule_all_then assume_tac)
-        \\ gvs [])
-      >- ((* Seq *)
-        IF_CASES_TAC \\ fs []
-        \\ gvs [LENGTH_EQ_NUM_compute]
-        \\ cheat (* TODO *))))
+        \\ gvs [])))
 QED
 
 val _ = export_theory ();
